theories/Factor_Finite_Equality_Source.thy
@@ -1,0 +1,47 @@
+theory Factor_Finite_Equality_Source
+  imports Factor_Native_Equality Factor_Finite_Artifact_Enumeration Factor_Executable_Systems
+begin
+
+section \<open>A finite presentation of the existing complete equality source\<close>
+
+definition finite_equality_artifact :: finite_exact_artifact where
+  "finite_equality_artifact=finite_enumerated_artifact (map (\<lambda>n. [n]) [0..<26])
+    (map (\<lambda>(r,s,t). ([r],[s],[t]))
+      [(0,16,15),(15,15,1),(1,17,2),(1,18,6),(17,17,18),
+       (2,19,3),(2,20,5),(19,19,20),(3,4,4),(5,5,4),
+       (6,7,8),(8,21,9),(8,22,11),(8,23,14),(21,21,22),(22,22,23),
+       (9,10,10),(11,24,12),(11,25,13),(24,24,25),(12,12,10),(13,13,10)]) [] []"
+
+theorem finite_equality_artifact_correct:
+  "decode_finite_object finite_equality_artifact=equality_artifact"
+  by (auto simp: finite_equality_artifact_def equality_artifact_def finite_enumerated_artifact_def
+    decode_finite_object_def decode_finite_structure_def decode_finite_basis_def empty_basis_def
+    fset_of_list.rep_eq fun_eq_iff)
+
+definition finite_equality_environment :: "local_address option finite_artifact_environment" where
+  "finite_equality_environment=finite_enumerated_environment [(None,finite_equality_artifact)] []"
+
+lemma finite_equality_environment_correct:
+  "decode_finite_environment finite_equality_environment=equality_environment"
+  by (simp add: finite_equality_environment_def finite_equality_artifact_correct equality_environment_def
+    literal_environment_def map_relation_values_def)
+
+lemma finite_equality_environment_formed:
+  "finite_environment_formed finite_equality_environment"
+  by (simp only: finite_environment_formed_correct finite_equality_environment_correct equality_environment_formed)
+
+definition finite_equality_schema ::
+  "(local_address,local_address,local_address option definition_site) finite_factor_schema" where
+  "finite_equality_schema=\<lparr>finite_schema_conclusion=Finite_Pattern_Pair (Finite_Variable [10]) (Finite_Variable [10]),
+    finite_schema_premises={||},finite_schema_materials={||}\<rparr>"
+
+lemma finite_equality_schema_correct:
+  "decode_finite_schema finite_equality_schema=native_equality_schema"
+  by (simp add: finite_equality_schema_def native_equality_schema_def decode_finite_schema_def map_relation_values_def)
+
+text \<open>
+  The finite rows recover exactly the original equality artifact, environment,
+  and schema. They introduce no replacement meaning for the original program.
+\<close>
+
+end
