theories/Factor_Requirement_Source_Examples.thy
@@ -1,0 +1,203 @@
+theory Factor_Requirement_Source_Examples
+  imports Factor_Requirement_Source_Readings Factor_Requirement_Packages Factor_Selected_Definition_Graphs
+begin
+
+section \<open>Complete native packages are recovered from the executed source artifacts\<close>
+
+definition finite_guard_source_program :: "bool \<Rightarrow> local_address option finite_native_system" where
+  "finite_guard_source_program b=\<lparr>
+    finite_system_interfaces={|((None,[Suc 0]),Finite_Variable [4])|},
+    finite_system_clauses={|(((None,[Suc 0]),[7]),if b then finite_variable_schema else finite_equality_schema)|}\<rparr>"
+
+definition finite_guard_program :: "bool \<Rightarrow> local_address option finite_native_system" where
+  "finite_guard_program b=\<lparr>
+    finite_system_interfaces={|((None,[Suc 0]),Finite_Variable [4]),((Some [Suc 0],[Suc 0]),Finite_Variable [4])|},
+    finite_system_clauses={|(((None,[Suc 0]),[7]),if b then finite_variable_schema else finite_equality_schema),
+      (((Some [Suc 0],[Suc 0]),[7]),finite_guard_schema)|}\<rparr>"
+
+lemma finite_guard_source_included:
+  "environment_included (decode_finite_environment (finite_guard_source b))
+    (decode_finite_environment (finite_guard_environment b))"
+  by (auto simp: finite_guard_source_def finite_guard_environment_def environment_included_def map_relation_values_def)
+
+lemma finite_guard_source_dependencies [simp]:
+  "schema_dependencies (decode_finite_schema finite_variable_schema)={}"
+  "schema_dependencies (decode_finite_schema finite_equality_schema)={}"
+  by (simp add: finite_variable_schema_def finite_equality_schema_def schema_dependencies_def rel_ran_def)+
+
+lemma finite_guard_source_choice_dependencies [simp]:
+  "schema_dependencies (decode_finite_schema (if b then finite_variable_schema else finite_equality_schema))={}"
+  by (cases b) simp_all
+
+lemma finite_guard_dependencies [simp]:
+  "schema_dependencies (decode_finite_schema finite_guard_schema)={(None,[Suc 0])}"
+  by (auto simp: finite_guard_schema_def finite_variable_schema_def schema_dependencies_def rel_ran_def map_relation_values_def)
+
+lemma finite_guard_source_package:
+  "native_package_at (decode_finite_environment (finite_guard_source b)) None [0]
+    (decode_finite_system (finite_guard_source_program b))"
+proof -
+  let ?E="decode_finite_environment (finite_guard_source b)"
+  let ?S="decode_finite_schema (if b then finite_variable_schema else finite_equality_schema)"
+  let ?G="{((None,[Suc 0]),Pattern_Variable [4],{([7],?S)})}
+    ::(local_address option definition_site \<times> local_address term_pattern \<times>
+      (local_address \<times> local_address option native_schema) set) set"
+  have ef: "environment_formed ?E" using finite_guard_environments_formed(1)[where b=b]
+    by (simp only: finite_environment_formed_correct)
+  have domain: "rel_dom ?G={(None,[Suc 0])}" by (auto simp: rel_dom_def)
+  have reads: "native_definition_at ?E (fst d) (snd d) p C" if "(d,p,C)\<in>?G" for d p C
+    using that finite_source_definition[where b=b] by auto
+  have closed: "schema_dependencies S\<subseteq>rel_dom ?G" if "(d,p,C)\<in>?G" "(c,S)\<in>C" for d p C c S
+    using that by auto
+  have graph: "native_package_formed ?E {(None,[Suc 0])}" "native_definition_graph ?E {(None,[Suc 0])}=?G"
+    using native_closed_definition_graph(2,3)[OF ef reads closed] by (simp_all only: domain)
+  have program: "native_program ?E {(None,[Suc 0])}=decode_finite_system (finite_guard_source_program b)"
+    by (simp only: native_program_def graph(2);
+      auto simp: finite_guard_source_program_def decode_finite_system_def map_relation_values_def)
+  have roots: "native_root_family_at ?E None [0] {([16],(None,[Suc 0]))}"
+    using finite_guard_source_roots[where b=b] by simp
+  show ?thesis unfolding native_package_at_def
+    by (rule exI[of _ "{([16],(None,[Suc 0]))}"]) (use roots graph(1) program in \<open>auto simp: rel_ran_def\<close>)
+qed
+
+lemma finite_guard_package:
+  "native_package_at (decode_finite_environment (finite_guard_environment b)) (Some [Suc 0]) [0]
+    (decode_finite_system (finite_guard_program b))"
+proof -
+  let ?E="decode_finite_environment (finite_guard_environment b)"
+  let ?S="decode_finite_schema (if b then finite_variable_schema else finite_equality_schema)"
+  let ?T="decode_finite_schema finite_guard_schema"
+  let ?k="(None,[Suc 0])" let ?g="(Some [Suc 0],[Suc 0])"
+  let ?G="{(?k,Pattern_Variable [4],{([7],?S)}),(?g,Pattern_Variable [4],{([7],?T)})}
+    ::(local_address option definition_site \<times> local_address term_pattern \<times>
+      (local_address \<times> local_address option native_schema) set) set"
+  have ef: "environment_formed ?E" using finite_guard_environments_formed(2)[where b=b]
+    by (simp only: finite_environment_formed_correct)
+  have old: "native_definition_at ?E None [Suc 0] (Pattern_Variable [4]) {([7],?S)}"
+    using native_definition_included[OF finite_source_definition[where b=b]
+      finite_guard_source_included[where b=b] ef] by simp
+  have raw: "native_definition_at ?E (Some [Suc 0]) [Suc 0] (Pattern_Variable [4]) {([7],?T)}"
+    using finite_guard_raw_definition[where b=b] by simp
+  have domain: "rel_dom ?G={?k,?g}" by (auto simp: rel_dom_def)
+  have reads: "native_definition_at ?E (fst d) (snd d) p C" if "(d,p,C)\<in>?G" for d p C
+    using that old raw by auto
+  have closed: "schema_dependencies S\<subseteq>rel_dom ?G" if "(d,p,C)\<in>?G" "(c,S)\<in>C" for d p C c S
+    using that by (auto simp: domain)
+  have start: "?g\<in>native_definition_sites ?E {?g}" using native_definition_roots[of "{?g}" ?E] by auto
+  have edge: "(?g,?k)\<in>native_definition_edges ?E"
+    by (simp only: native_definition_edges_at[OF raw]; auto)
+  have reached: "?k\<in>native_definition_sites ?E {?g}" by (rule native_definition_step[OF start edge])
+  have roots_inside: "{?g}\<subseteq>rel_dom ?G" by (simp add: domain)
+  have coverage: "rel_dom ?G\<subseteq>native_definition_sites ?E {?g}" using start reached by (simp add: domain)
+  have package: "native_package_formed ?E {?g}"
+    by (rule native_selected_definition_graph(2)[OF ef reads closed roots_inside coverage])
+  have graph: "native_definition_graph ?E {?g}=?G"
+    by (rule native_selected_definition_graph(3)[OF ef reads closed roots_inside coverage])
+  have program: "native_program ?E {?g}=decode_finite_system (finite_guard_program b)"
+    by (simp only: native_program_def graph;
+      auto simp: finite_guard_program_def decode_finite_system_def map_relation_values_def)
+  have roots: "native_root_family_at ?E (Some [Suc 0]) [0] {([16],?g)}"
+    using finite_guard_roots[where b=b] by simp
+  show ?thesis unfolding native_package_at_def
+    by (rule exI[of _ "{([16],?g)}"]) (use roots package program in \<open>auto simp: rel_ran_def\<close>)
+qed
+
+lemma finite_guard_definition:
+  "native_single_clause_at (decode_finite_environment (finite_guard_environment b)) (Some [Suc 0]) [Suc 0]
+    (decode_finite_schema finite_guard_schema)"
+  using finite_guard_raw_definition[where b=b] by (auto simp: native_single_clause_at_def)
+
+lemma finite_variable_definition:
+  "native_single_clause_at (decode_finite_environment (finite_guard_source True)) None [Suc 0]
+    (decode_finite_schema finite_variable_schema)"
+  using finite_source_definition[where b=True] by (auto simp: native_single_clause_at_def)
+
+lemma finite_guard_source_definitions [simp]:
+  "system_definitions (decode_finite_system (finite_guard_source_program b))={(None,[Suc 0])}"
+  by (auto simp: finite_guard_source_program_def system_definitions_def rel_dom_def map_relation_values_def)
+
+lemma finite_guard_definitions [simp]:
+  "system_definitions (decode_finite_system (finite_guard_program b))={(None,[Suc 0]),(Some [Suc 0],[Suc 0])}"
+  by (auto simp: finite_guard_program_def system_definitions_def rel_dom_def map_relation_values_def)
+
+section \<open>The same guard calls different meanings at the same actual source site\<close>
+
+lemma finite_variable_requirement_schema:
+  "schema_alpha_variant (requirement_guard_schema ({}::(nat\<times>local_address option definition_site) set))
+    (decode_finite_schema finite_variable_schema)"
+  unfolding schema_alpha_variant_def
+  by (rule exI[of _ "\<lambda>_. [10]"], rule exI[of _ "\<lambda>_. [26]"])
+    (auto simp: finite_variable_schema_def finite_equality_schema_def decode_finite_schema_def
+      requirement_guard_schema_def schema_variables_def schema_sockets_def rel_dom_def rename_schema_def map_socket_graph_def map_relation_values_def)
+
+lemma finite_guard_requirement_schema:
+  "schema_alpha_variant (requirement_guard_schema {(0::nat,(None,[Suc 0]))})
+    (decode_finite_schema finite_guard_schema)"
+  unfolding schema_alpha_variant_def
+  by (rule exI[of _ "\<lambda>_. [10]"], rule exI[of _ "\<lambda>_. [26]"])
+    (auto simp: finite_guard_schema_def finite_variable_schema_def finite_equality_schema_def decode_finite_schema_def
+      requirement_guard_schema_def schema_variables_def schema_sockets_def rel_dom_def rename_schema_def map_socket_graph_def map_relation_values_def)
+
+theorem finite_guard_source_meaning:
+  "((None,[Suc 0]),t)\<in>positive_meaning (decode_finite_system (finite_guard_source_program b)) \<longleftrightarrow>
+    (if b then term_formed t else (\<exists>x. term_formed x \<and> t=Pair_Term x x))"
+proof (cases b)
+  case False
+  have same: "decode_finite_system (finite_guard_source_program False)=native_equality_program"
+    by (simp add: finite_guard_source_program_def native_equality_program_def decode_finite_system_def
+      finite_equality_schema_correct map_relation_values_def)
+  show ?thesis using native_equality_exact[of t] by (simp only: False same; simp)
+next
+  case True
+  have member: "(None,[Suc 0])\<in>system_definitions (decode_finite_system (finite_guard_source_program True))" by simp
+  have read: "native_single_clause_at (decode_finite_environment (finite_guard_source True))
+      (fst (None,[Suc 0])) (snd (None,[Suc 0])) (decode_finite_schema finite_variable_schema)"
+    using finite_variable_definition by simp
+  have actual: "((None,[Suc 0]),t)\<in>positive_meaning (decode_finite_system (finite_guard_source_program True))
+      \<longleftrightarrow> term_formed t \<and>
+        (\<forall>(s,k)\<in>({}::(nat\<times>local_address option definition_site) set).
+          (k,t)\<in>positive_meaning (decode_finite_system (finite_guard_source_program True)))"
+    by (rule native_requirement_meaning[OF finite_guard_source_package[where b=True] _
+        finite_guard_source_package[where b=True] member read finite_variable_requirement_schema])
+      (auto simp: environment_included_def single_valued_def rel_ran_def)
+  show ?thesis using actual by (simp only: True; simp)
+qed
+
+theorem finite_guard_program_meaning:
+  "((Some [Suc 0],[Suc 0]),t)\<in>positive_meaning (decode_finite_system (finite_guard_program b)) \<longleftrightarrow>
+    (if b then term_formed t else (\<exists>x. term_formed x \<and> t=Pair_Term x x))"
+proof -
+  have member: "(Some [Suc 0],[Suc 0])\<in>system_definitions (decode_finite_system (finite_guard_program b))" by simp
+  have read: "native_single_clause_at (decode_finite_environment (finite_guard_environment b))
+      (fst (Some [Suc 0],[Suc 0])) (snd (Some [Suc 0],[Suc 0])) (decode_finite_schema finite_guard_schema)"
+    using finite_guard_definition by simp
+  have actual: "((Some [Suc 0],[Suc 0]),t)\<in>positive_meaning (decode_finite_system (finite_guard_program b)) \<longleftrightarrow>
+      term_formed t \<and> (\<forall>(s,k)\<in>{(0::nat,(None,[Suc 0]))}.
+        (k,t)\<in>positive_meaning (decode_finite_system (finite_guard_source_program b)))"
+    by (rule native_requirement_meaning[OF finite_guard_source_package finite_guard_source_included
+        finite_guard_package member read finite_guard_requirement_schema])
+      (auto simp: single_valued_def rel_ran_def)
+  show ?thesis by (simp only: actual; auto simp: finite_guard_source_meaning split: if_splits)
+qed
+
+definition native_guard_source_meaning_report where
+  "native_guard_source_meaning_report b=(
+    sorted_list_of_set (system_definitions (decode_finite_system (finite_guard_program b))),
+    ((Some [Suc 0],[Suc 0]),Payload_Term [])\<in>positive_meaning (decode_finite_system (finite_guard_program b)))"
+
+lemma native_guard_source_meaning_report_code [code]:
+  "native_guard_source_meaning_report b=([(None,[Suc 0]),(Some [Suc 0],[Suc 0])],b)"
+  by (simp add: native_guard_source_meaning_report_def finite_guard_program_meaning octets_formed_def)
+
+export_code native_guard_source_meaning_report integer_of_nat
+  in SML module_name Native_Guard_Source_Meaning file_prefix native_guard_source_meaning
+
+text \<open>
+  Complete native package recovery fixes both original source programs and
+  both installed programs. Their domains are equal, and the installed guard
+  schema is identical. Nevertheless, its meaning on the same empty payload
+  changes with the actual source clause. The source-retaining native checker
+  rejects that replacement under the original declared source.
+\<close>
+
+end
