theories/Factor_Requirement_Source_Readings.thy
@@ -1,0 +1,287 @@
+theory Factor_Requirement_Source_Readings
+  imports Retained_Clause_Execution
+begin
+
+section \<open>Both executed artifacts use the same complete variable frame\<close>
+
+abbreviation finite_requirement_frame where
+  "finite_requirement_frame b \<equiv> if b then finite_guard_artifact else finite_variable_artifact"
+
+lemma finite_requirement_frame_records:
+  assumes formed: "finite_object_formed (finite_requirement_frame b)"
+  shows "finite_record_at (finite_requirement_frame b) [1] [[17],[18]] [[2],[6]]"
+  "finite_record_at (finite_requirement_frame b) [2] [[19],[20]] [[3],[5]]"
+  "finite_record_at (finite_requirement_frame b) [8] [[21],[22],[23]] [[9],[11],[14]]"
+  by (simp only: finite_record_at_def formed; cases b; simp_all only: if_True if_False; code_simp)+
+
+lemma finite_requirement_frame_families:
+  assumes formed: "finite_object_formed (finite_requirement_frame b)"
+  shows "finite_family_at (finite_requirement_frame b) [0] {|([16],[15])|}"
+  "finite_family_at (finite_requirement_frame b) [6] {|([7],[8])|}"
+  "finite_binder_scope_at (finite_requirement_frame b) [3] {|[4]|}"
+  "finite_binder_scope_at (finite_requirement_frame b) [9] {|[10]|}"
+  by (simp only: finite_binder_scope_at_def finite_family_at_def formed; cases b; simp_all only: if_True if_False; code_simp)+
+
+lemma finite_requirement_frame_citations:
+  assumes formed: "finite_exact_formed (finite_requirement_frame b)"
+  shows "finite_citation_at (finite_requirement_frame b) [5] (Local [4]) {|[5]|}"
+  "finite_citation_at (finite_requirement_frame b) [11] (Local [10]) {|[11]|}"
+  "finite_citation_at (finite_requirement_frame b) [15] (Local [1]) {|[15]|}"
+  by (simp only: finite_citation_at_def formed; cases b; simp_all only: if_True if_False; code_simp)+
+
+lemma finite_requirement_frame_carrier:
+  "[1] |\<in>| finite_carrier (finite_structure (finite_requirement_frame b))"
+  by (cases b; simp_all only: if_True if_False; code_simp)
+
+locale requirement_source_frame =
+  fixes E :: "'u artifact_environment" and u :: 'u and b :: bool
+  assumes formed: "environment_formed E"
+    and artifact: "artifact_at E u (decode_finite_object (finite_requirement_frame b))"
+begin
+
+lemma finite_exact: "finite_exact_formed (finite_requirement_frame b)"
+  using formed artifact by (simp add: finite_exact_formed_correct environment_formed_def)
+
+lemma finite_object: "finite_object_formed (finite_requirement_frame b)"
+  using finite_exact by (simp add: finite_exact_formed_def)
+
+lemma interface:
+  "scoped_pattern_at E u [2] (Pattern_Variable [4]) {[2],[19],[20],[3],[4],[5]} {}"
+proof -
+  let ?A="decode_finite_object (finite_requirement_frame b)"
+  have rec: "record_at ?A [2] [[19],[20]] [[3],[5]]"
+    using finite_requirement_frame_records(2)[OF finite_object] by (simp only: finite_record_at_correct)
+  have scope: "binder_scope_at ?A [3] {[4]}"
+    using finite_requirement_frame_families(3)[OF finite_object] by (simp add: finite_binder_scope_at_correct)
+  have cite: "citation_at ?A [5] (Local [4]) {[5]}"
+    using finite_requirement_frame_citations(1)[OF finite_exact] by (simp add: finite_citation_at_correct)
+  have quote: "pattern_quoted_at E u {[4]} [5] (Pattern_Variable [4]) {[5]} {}"
+    by (rule pattern_quoted_at.variable[OF formed artifact cite]) auto
+  show ?thesis unfolding scoped_pattern_at_def
+    by (rule conjI[OF formed], rule exI[of _ ?A], rule exI[of _ "[[19],[20]]"],
+      rule exI[of _ "[3]"], rule exI[of _ "[5]"], rule exI[of _ "{[4]}"], rule exI[of _ "{[5]}"])
+      (use artifact rec scope quote in auto)
+qed
+
+lemma schema:
+  assumes conclusion: "schema_conclusion S=Pattern_Variable [10]"
+    and variables: "schema_variables S={[10]}" and material: "schema_material_premises S={}"
+    and calls: "prospective_family_at E u {[10]} [14] (schema_premises S)"
+  shows "native_schema_at E u [8] S"
+proof -
+  let ?A="decode_finite_object (finite_requirement_frame b)"
+  have rec: "record_at ?A [8] [[21],[22],[23]] [[9],[11],[14]]"
+    using finite_requirement_frame_records(3)[OF finite_object] by (simp only: finite_record_at_correct)
+  have scope: "binder_scope_at ?A [9] {[10]}"
+    using finite_requirement_frame_families(4)[OF finite_object] by (simp add: finite_binder_scope_at_correct)
+  have cite: "citation_at ?A [11] (Local [10]) {[11]}"
+    using finite_requirement_frame_citations(2)[OF finite_exact] by (simp add: finite_citation_at_correct)
+  have quote: "pattern_quoted_at E u {[10]} [11] (Pattern_Variable [10]) {[11]} {}"
+    by (rule pattern_quoted_at.variable[OF formed artifact cite]) auto
+  show ?thesis unfolding native_schema_at_def
+    by (rule conjI[OF formed], rule exI[of _ ?A], rule exI[of _ "[[21],[22],[23]]"],
+      rule exI[of _ "[9]"], rule exI[of _ "[11]"], rule exI[of _ "[14]"],
+      rule exI[of _ "{[10]}"], rule exI[of _ "{[11]}"], rule exI[of _ "{}"])
+      (use artifact rec scope quote calls conclusion variables material in
+        \<open>auto simp: native_premise_family_calls_only\<close>)
+qed
+
+lemma raw_definition:
+  assumes schema: "native_schema_at E u [8] S"
+  shows "native_definition_at E u [1] (Pattern_Variable [4]) {([7],S)}"
+proof -
+  let ?A="decode_finite_object (finite_requirement_frame b)"
+  have rec: "record_at ?A [1] [[17],[18]] [[2],[6]]"
+    using finite_requirement_frame_records(1)[OF finite_object] by (simp only: finite_record_at_correct)
+  have family: "family_at ?A [6] {([7],[8])}"
+    using finite_requirement_frame_families(2)[OF finite_object] by (simp add: finite_family_at_correct)
+  have clauses: "native_schema_family_at E u [6] {([7],S)}"
+    unfolding native_schema_family_at_def
+    by (rule conjI[OF formed], rule exI[of _ ?A], rule exI[of _ "{([7],[8])}"])
+      (use artifact family schema in \<open>auto simp: single_valued_def rel_dom_def\<close>)
+  show ?thesis unfolding native_definition_at_def
+    by (rule conjI[OF formed], rule exI[of _ ?A], rule exI[of _ "[[17],[18]]"],
+      rule exI[of _ "[2]"], rule exI[of _ "[6]"],
+      rule exI[of _ "{[2],[19],[20],[3],[4],[5]}"], rule exI[of _ "{}"])
+      (use artifact rec interface clauses in auto)
+qed
+
+lemma roots: "native_root_family_at E u [0] {([16],(u,[1]))}"
+proof -
+  let ?A="decode_finite_object (finite_requirement_frame b)"
+  have family: "family_at ?A [0] {([16],[15])}"
+    using finite_requirement_frame_families(1)[OF finite_object] by (simp add: finite_family_at_correct)
+  have cite: "citation_at ?A [15] (Local [1]) {[15]}"
+    using finite_requirement_frame_citations(3)[OF finite_exact] by (simp add: finite_citation_at_correct)
+  have af: "exact_formed ?A" using formed artifact by (simp add: environment_formed_def)
+  have carrier: "[1]\<in>rra_carrier (object_structure ?A)"
+    using finite_requirement_frame_carrier[where b=b] by (simp add: decode_finite_object_def decode_finite_structure_def)
+  have location: "citation_location E u (Local [1]) u [1]"
+    using artifact af carrier by (auto simp: anchor_formed_def)
+  have loc: "located_at E u [15] u [1]" using artifact cite location unfolding located_at_def by blast
+  show ?thesis unfolding native_root_family_at_def
+    by (rule conjI[OF formed], rule exI[of _ ?A], rule exI[of _ "{([16],[15])}"])
+      (use artifact family loc in \<open>auto simp: single_valued_def rel_dom_def\<close>)
+qed
+
+end
+
+lemma finite_guard_environments_formed:
+  "finite_environment_formed (finite_guard_source b)"
+  "finite_environment_formed (finite_guard_environment b)"
+  by (cases b; simp_all only: if_True if_False; code_simp)+
+
+lemma finite_variable_source_frame:
+  "requirement_source_frame (decode_finite_environment (finite_guard_source True)) None False"
+  by (rule requirement_source_frame.intro)
+    (use finite_guard_environments_formed(1)[where b=True] in
+      \<open>auto simp: finite_environment_formed_correct finite_guard_source_def artifact_at_def map_relation_values_def\<close>)
+
+lemma finite_guard_frame:
+  "requirement_source_frame (decode_finite_environment (finite_guard_environment b)) (Some [1]) True"
+  by (rule requirement_source_frame.intro)
+    (use finite_guard_environments_formed(2)[where b=b] in
+      \<open>auto simp: finite_environment_formed_correct finite_guard_environment_def artifact_at_def map_relation_values_def\<close>)
+
+lemma finite_variable_premise_check: "finite_family_at finite_variable_artifact [14] {||}"
+  by code_simp
+
+lemma finite_variable_source_schema:
+  "native_schema_at (decode_finite_environment (finite_guard_source True)) None [8]
+    (decode_finite_schema finite_variable_schema)"
+proof -
+  interpret frame: requirement_source_frame "decode_finite_environment (finite_guard_source True)" None False
+    by (rule finite_variable_source_frame)
+  have family: "family_at (decode_finite_object finite_variable_artifact) [14] {}"
+    using finite_variable_premise_check by (simp add: finite_family_at_correct)
+  have body: "prospective_family_at (decode_finite_environment (finite_guard_source True)) None {[10]} [14] {}"
+    unfolding prospective_family_at_def
+    by (rule conjI[OF frame.formed], rule exI[of _ "decode_finite_object finite_variable_artifact"], rule exI[of _ "{}"])
+      (use frame.artifact family in \<open>auto simp: single_valued_def rel_dom_def\<close>)
+  show ?thesis by (rule frame.schema)
+    (use body in \<open>auto simp: finite_variable_schema_def finite_equality_schema_def decode_finite_schema_def
+      schema_variables_def rel_ran_def map_relation_values_def\<close>)
+qed
+
+lemma finite_guard_premise_checks:
+  "finite_record_at finite_guard_artifact [27] [[28],[29]] [[30],[31]]"
+  "finite_family_at finite_guard_artifact [14] {|([26],[27])|}"
+  "finite_citation_at finite_guard_artifact [31] (Local [10]) {|[31]|}"
+  "finite_citation_at finite_guard_artifact [30] (External [32] [1]) {|[30],[33]|}"
+proof -
+  have exact: "finite_exact_formed finite_guard_artifact"
+    using requirement_source_frame.finite_exact[OF finite_guard_frame[where b=False]] by simp
+  have formed: "finite_object_formed finite_guard_artifact" using exact by (simp add: finite_exact_formed_def)
+  show "finite_record_at finite_guard_artifact [27] [[28],[29]] [[30],[31]]"
+    by (simp only: finite_record_at_def formed; code_simp)
+  show "finite_family_at finite_guard_artifact [14] {|([26],[27])|}"
+    by (simp only: finite_family_at_def formed; code_simp)
+  show "finite_citation_at finite_guard_artifact [31] (Local [10]) {|[31]|}"
+    by (simp only: finite_citation_at_def exact; code_simp)
+  show "finite_citation_at finite_guard_artifact [30] (External [32] [1]) {|[30],[33]|}"
+    by (simp only: finite_citation_at_def exact; code_simp)
+qed
+
+lemma finite_guard_source_carrier:
+  "[1] |\<in>| finite_carrier (finite_structure (if b then finite_variable_artifact else finite_equality_artifact))"
+  by (cases b; simp_all only: if_True if_False; code_simp)
+
+lemma finite_guard_prospective:
+  "prospective_call_at (decode_finite_environment (finite_guard_environment b)) (Some [1]) {[10]} [27]
+    (None,[1]) (Pattern_Variable [10]) {[27],[28],[29],[30],[33],[31]} {[32]}"
+proof -
+  interpret frame: requirement_source_frame "decode_finite_environment (finite_guard_environment b)" "Some [1]" True
+    by (rule finite_guard_frame)
+  let ?E="decode_finite_environment (finite_guard_environment b)"
+  let ?A="decode_finite_object finite_guard_artifact"
+  have rec: "record_at ?A [27] [[28],[29]] [[30],[31]]"
+    using finite_guard_premise_checks(1) by (simp only: finite_record_at_correct)
+  have variable: "citation_at ?A [31] (Local [10]) {[31]}"
+    using finite_guard_premise_checks(3) by (simp add: finite_citation_at_correct)
+  have art: "artifact_at ?E (Some [1]) ?A" using frame.artifact by simp
+  have quote: "pattern_quoted_at ?E (Some [1]) {[10]} [31] (Pattern_Variable [10]) {[31]} {}"
+    by (rule pattern_quoted_at.variable[OF frame.formed art variable]) auto
+  let ?cite="External [32] [1]"
+  have citation: "citation_at ?A [30] ?cite {[30],[33]}"
+    using finite_guard_premise_checks(4) by (simp add: finite_citation_at_correct)
+  let ?source="decode_finite_object (if b then finite_variable_artifact else finite_equality_artifact)"
+  have source: "artifact_at ?E None ?source"
+    by (simp add: finite_guard_environment_def artifact_at_def map_relation_values_def)
+  have exact: "exact_formed ?source" using frame.formed source by (simp add: environment_formed_def)
+  have carrier: "[1]\<in>rra_carrier (object_structure ?source)"
+    using finite_guard_source_carrier[where b=b] by simp
+  have binding: "binds_slot ?E (Some [1]) [32] None"
+    by (simp add: finite_guard_environment_def binds_slot_def)
+  have loc: "citation_location ?E (Some [1]) ?cite None [1]"
+    using source exact carrier binding by (auto simp: anchor_formed_def)
+  have slots: "citation_slots ?cite={[32]}" by simp
+  show ?thesis unfolding prospective_call_at_def
+    by (rule conjI[OF frame.formed], rule exI[of _ ?A], rule exI[of _ "[[28],[29]]"],
+      rule exI[of _ "[30]"], rule exI[of _ "[31]"], rule exI[of _ ?cite],
+      rule exI[of _ "{[30],[33]}"], rule exI[of _ "{[31]}"], rule exI[of _ "{}"])
+      (use art rec citation loc quote slots in \<open>simp add: insert_commute\<close>)
+qed
+
+lemma finite_guard_native_schema:
+  "native_schema_at (decode_finite_environment (finite_guard_environment b)) (Some [1]) [8]
+    (decode_finite_schema finite_guard_schema)"
+proof -
+  interpret frame: requirement_source_frame "decode_finite_environment (finite_guard_environment b)" "Some [1]" True
+    by (rule finite_guard_frame)
+  have family: "family_at (decode_finite_object finite_guard_artifact) [14] {([26],[27])}"
+    using finite_guard_premise_checks(2) by (simp add: finite_family_at_correct)
+  have body: "prospective_family_at (decode_finite_environment (finite_guard_environment b)) (Some [1]) {[10]} [14]
+      {([26],(None,[1]),Pattern_Variable [10])}"
+    unfolding prospective_family_at_def
+    by (rule conjI[OF frame.formed], rule exI[of _ "decode_finite_object finite_guard_artifact"],
+      rule exI[of _ "{([26],[27])}"])
+      (use frame.artifact family finite_guard_prospective[where b=b] in \<open>auto simp: single_valued_def rel_dom_def\<close>)
+  show ?thesis by (rule frame.schema)
+    (use body in \<open>auto simp: finite_guard_schema_def finite_variable_schema_def finite_equality_schema_def
+      decode_finite_schema_def schema_variables_def rel_ran_def map_relation_values_def\<close>)
+qed
+
+lemma finite_source_definition:
+  "native_definition_at (decode_finite_environment (finite_guard_source b)) None [1]
+    (Pattern_Variable [4]) {([7],decode_finite_schema (if b then finite_variable_schema else finite_equality_schema))}"
+proof (cases b)
+  case False
+  have same: "decode_finite_environment (finite_guard_source False)=equality_environment"
+    by (simp add: finite_guard_source_def finite_equality_environment_def[symmetric] finite_equality_environment_correct)
+  show ?thesis using equality_definition_at by (simp only: False if_False same finite_equality_schema_correct; simp)
+next
+  case True
+  show ?thesis using requirement_source_frame.raw_definition[OF finite_variable_source_frame finite_variable_source_schema]
+    by (simp only: True if_True)
+qed
+
+lemma finite_guard_raw_definition:
+  "native_definition_at (decode_finite_environment (finite_guard_environment b)) (Some [1]) [1]
+    (Pattern_Variable [4]) {([7],decode_finite_schema finite_guard_schema)}"
+  by (rule requirement_source_frame.raw_definition[OF finite_guard_frame finite_guard_native_schema])
+
+lemma finite_guard_source_roots:
+  "native_root_family_at (decode_finite_environment (finite_guard_source b)) None [0] {([16],(None,[1]))}"
+proof (cases b)
+  case False
+  show ?thesis using equality_root_family
+    by (simp only: False; simp add: finite_guard_source_def finite_equality_environment_def[symmetric]
+      finite_equality_environment_correct)
+next
+  case True
+  show ?thesis using requirement_source_frame.roots[OF finite_variable_source_frame] by (simp only: True)
+qed
+
+lemma finite_guard_roots:
+  "native_root_family_at (decode_finite_environment (finite_guard_environment b)) (Some [1]) [0]
+    {([16],(Some [1],[1]))}"
+  by (rule requirement_source_frame.roots[OF finite_guard_frame])
+
+text \<open>
+  The two executed artifacts share one concrete frame. Its complete interface,
+  schema, definition, and roots are recovered once with arbitrary surrounding
+  environment and use. The variable and guarded instances supply their actual
+  premise families. The unchanged equality instance reuses its original proof.
+\<close>
+
+end
