theories/Factor_Retained_Clause_Admission.thy
@@ -1,0 +1,258 @@
+theory Factor_Retained_Clause_Admission
+  imports Factor_Related_Test_Admission
+begin
+
+section \<open>One actual package entry retains its source and complete clause\<close>
+
+definition retained_clause_schema :: "factor_term \<Rightarrow> factor_term \<Rightarrow> (nat,nat,nat) factor_schema" where
+  "retained_clause_schema e v=data_rule
+    (package_subject_pattern data_x data_y data_z data_w)
+    {(0,83,package_subject_pattern data_x data_y data_z data_w),
+     (1,113,Pattern_Pair (exact_term_pattern e) data_x),
+     (2,127,Pattern_Pair (Pattern_Pair data_x data_w) (exact_term_pattern v))}"
+
+definition retained_clause_system :: "factor_term \<Rightarrow> factor_term \<Rightarrow> (nat,nat,nat,nat) schema_system" where
+  "retained_clause_system e v=add_view_definition related_test_admission_base 370 data_x
+    {(0,retained_clause_schema e v)}"
+
+definition retained_clause_result where
+  "retained_clause_result E S p \<longleftrightarrow>
+    (\<exists>F u r Q d f. environment_value_presents F f \<and>
+      p=package_subject_argument f (use_data_term u) (Payload_Term r) (definition_site_value d) \<and>
+      native_package_at F u r Q \<and> d\<in>system_definitions Q \<and>
+      environment_included E F \<and> native_single_clause_at F (fst d) (snd d) S)"
+
+locale retained_clause_reader =
+  fixes e v :: factor_term
+  assumes fields: "term_formed e" "term_formed v"
+begin
+
+lemma schema_formed: "schema_formed (retained_clause_schema e v)"
+  using fields by (auto simp: retained_clause_schema_def schema_formed_def single_valued_def)
+
+lemma dependencies: "schema_dependencies (retained_clause_schema e v)={83,113,127}"
+  by (simp add: retained_clause_schema_def schema_dependencies_def rel_ran_image)
+
+sublocale view: positive_view related_test_admission_base 370 data_x "{(0,retained_clause_schema e v)}"
+  by (rule positive_view.intro)
+    (use related_test_admission_base_bound related_test_admission_base_roots schema_formed dependencies
+      in \<open>auto simp: single_valued_def dest: subsetD\<close>)
+
+lemma formed: "schema_system_formed (retained_clause_system e v)"
+  using view.formed by (simp only: retained_clause_system_def)
+
+lemma definitions [simp]: "system_definitions (retained_clause_system e v)=
+  insert 370 (system_definitions related_test_admission_base)"
+  by (simp add: retained_clause_system_def)
+
+lemma calls: "schema_call_formed (retained_clause_system e v) d t \<longleftrightarrow>
+    d\<in>system_definitions (retained_clause_system e v) \<and> term_formed t"
+  using added_variable_calls[OF related_test_admission_base_formed view.formed related_test_admission_base_call]
+  by (simp only: retained_clause_system_def)
+
+lemma old_meaning:
+  assumes "d\<in>system_definitions related_test_admission_base"
+  shows "(d,t)\<in>positive_meaning (retained_clause_system e v) \<longleftrightarrow>
+    (d,t)\<in>positive_meaning related_test_admission_base"
+  using view.old_meaning[OF assms] by (simp only: retained_clause_system_def)
+
+lemma clause [simp]: "((370,c),S)\<in>system_clauses (retained_clause_system e v) \<longleftrightarrow>
+  c=0 \<and> S=retained_clause_schema e v"
+  using view.no_old_clause by (auto simp: retained_clause_system_def)
+
+lemma components:
+  "(83,t)\<in>positive_meaning (retained_clause_system e v) \<longleftrightarrow>
+    (83,t)\<in>positive_meaning package_membership_system"
+  "(113,t)\<in>positive_meaning (retained_clause_system e v) \<longleftrightarrow>
+    (113,t)\<in>positive_meaning environment_inclusion_system"
+  "(127,t)\<in>positive_meaning (retained_clause_system e v) \<longleftrightarrow>
+    (127,t)\<in>positive_meaning single_clause_reading_system"
+proof -
+  have retained: "d\<in>system_definitions related_test_admission_base" if "d\<in>{83,113,127}" for d
+    by (rule subsetD[OF related_test_admission_base_roots that])
+  have same: "(d,t)\<in>positive_meaning (retained_clause_system e v) \<longleftrightarrow>
+      (d,t)\<in>positive_meaning related_test_components_system" if "d\<in>{83,113,127}" for d
+    by (simp only: old_meaning[OF retained[OF that]] related_test_admission_base_meaning[OF retained[OF that]])
+  show "(83,t)\<in>positive_meaning (retained_clause_system e v) \<longleftrightarrow>
+    (83,t)\<in>positive_meaning package_membership_system" using same[of 83]
+    by (simp add: related_test_component_meanings)
+  show "(113,t)\<in>positive_meaning (retained_clause_system e v) \<longleftrightarrow>
+    (113,t)\<in>positive_meaning environment_inclusion_system" using same[of 113]
+    by (simp add: related_test_component_meanings)
+  show "(127,t)\<in>positive_meaning (retained_clause_system e v) \<longleftrightarrow>
+    (127,t)\<in>positive_meaning single_clause_reading_system" using same[of 127]
+    by (simp add: related_test_component_meanings)
+qed
+
+lemma valuation:
+  "(370,p)\<in>positive_meaning (retained_clause_system e v) \<longleftrightarrow>
+    (\<exists>h::nat\<Rightarrow>factor_term. (\<forall>j\<in>{0,1,2,3}. term_formed (h j)) \<and>
+      p=package_subject_argument (h 0) (h 1) (h 2) (h 3) \<and>
+      (83,p)\<in>positive_meaning package_membership_system \<and>
+      (113,Pair_Term e (h 0))\<in>positive_meaning environment_inclusion_system \<and>
+      (127,Pair_Term (Pair_Term (h 0) (h 3)) v)\<in>positive_meaning single_clause_reading_system)"
+proof -
+  have ordinary: "schema_material_premises (retained_clause_schema e v)={}"
+    by (simp add: retained_clause_schema_def)
+  have accepts: "schema_call_formed (retained_clause_system e v) 370
+      (evaluate_pattern h (schema_conclusion (retained_clause_schema e v)))"
+    if "\<forall>a\<in>schema_variables (retained_clause_schema e v). term_formed (h a)" for h
+    using that fields by (auto simp: calls retained_clause_schema_def schema_variables_def)
+  show ?thesis
+    apply (subst ordinary_single_clause_valuation[OF clause ordinary])
+    apply (rule accepts)
+    apply assumption
+    apply (rule ex_cong1)
+    using fields apply (auto simp: retained_clause_schema_def schema_variables_def components)
+    done
+qed
+
+lemma on_arguments:
+  "(370,package_subject_argument f u r d)\<in>positive_meaning (retained_clause_system e v) \<longleftrightarrow>
+    (83,package_subject_argument f u r d)\<in>positive_meaning package_membership_system \<and>
+    (113,Pair_Term e f)\<in>positive_meaning environment_inclusion_system \<and>
+    (127,Pair_Term (Pair_Term f d) v)\<in>positive_meaning single_clause_reading_system"
+proof
+  assume holds: "(370,package_subject_argument f u r d)\<in>positive_meaning (retained_clause_system e v)"
+  show "(83,package_subject_argument f u r d)\<in>positive_meaning package_membership_system \<and>
+    (113,Pair_Term e f)\<in>positive_meaning environment_inclusion_system \<and>
+    (127,Pair_Term (Pair_Term f d) v)\<in>positive_meaning single_clause_reading_system"
+    using holds by (auto simp: valuation)
+next
+  assume parts: "(83,package_subject_argument f u r d)\<in>positive_meaning package_membership_system \<and>
+    (113,Pair_Term e f)\<in>positive_meaning environment_inclusion_system \<and>
+    (127,Pair_Term (Pair_Term f d) v)\<in>positive_meaning single_clause_reading_system"
+  have formed: "term_formed f" "term_formed u" "term_formed r" "term_formed d"
+    using schema_call_formed_target[OF positive_meaning_formed[OF conjunct1[OF parts]]] by auto
+  let ?h="\<lambda>j::nat. if j=0 then f else if j=1 then u else if j=2 then r else d"
+  show "(370,package_subject_argument f u r d)\<in>positive_meaning (retained_clause_system e v)"
+    by (simp only: valuation; rule exI[of _ ?h]) (use formed parts in auto)
+qed
+
+theorem on_values:
+  assumes source: "environment_value_presents E e" and reference: "schema_reference_presents S v"
+    and target: "environment_value_presents F f"
+  shows "(370,package_subject_argument f (use_data_term u) (Payload_Term r) (definition_site_value d))
+      \<in>positive_meaning (retained_clause_system e v) \<longleftrightarrow>
+    (\<exists>Q. native_package_at F u r Q \<and> d\<in>system_definitions Q) \<and>
+      environment_included E F \<and> native_single_clause_at F (fst d) (snd d) S"
+proof -
+  have same: "G=E" if "environment_value_presents G e" for G
+    by (rule environment_value_presents_unique[OF that source])
+  have other: "G=F" if "environment_value_presents G f" for G
+    by (rule environment_value_presents_unique[OF that target])
+  have inclusion: "(113,Pair_Term e f)\<in>positive_meaning environment_inclusion_system \<longleftrightarrow>
+      environment_included E F"
+    by (simp only: environment_inclusion_exact factor_term.inject) (use source target same other in blast)
+  show ?thesis
+  proof (cases "\<exists>Q. native_package_at F u r Q \<and> d\<in>system_definitions Q")
+    case False
+    then show ?thesis by (simp only: on_arguments package_membership_on_values[OF target]; simp)
+  next
+    case True
+    then obtain Q where package: "native_package_at F u r Q" and member: "d\<in>system_definitions Q" by blast
+    have position: "d\<in>environment_positions F" by (rule native_package_entry_position[OF package member])
+    have site: "site_value_presents F (fst d) (snd d) (Pair_Term f (definition_site_value d))"
+      using target position by (simp add: site_value_presents_def site_data_term_def)
+    show ?thesis by (simp only: on_arguments package_membership_on_values[OF target] inclusion
+      single_clause_reading_at_reference[OF site reference])
+  qed
+qed
+
+theorem exact:
+  assumes source: "environment_value_presents E e" and reference: "schema_reference_presents S v"
+  shows "(370,p)\<in>positive_meaning (retained_clause_system e v) \<longleftrightarrow> retained_clause_result E S p"
+proof
+  assume holds: "(370,p)\<in>positive_meaning (retained_clause_system e v)"
+  have member: "(83,p)\<in>positive_meaning package_membership_system" using holds by (simp only: valuation; blast)
+  obtain F f u r d Q where parts: "environment_value_presents F f"
+    "p=package_subject_argument f (use_data_term u) (Payload_Term r) (definition_site_value d)"
+    "native_package_at F u r Q" "d\<in>system_definitions Q"
+    using package_membership_sound[OF member] by blast
+  have actual: "environment_included E F \<and> native_single_clause_at F (fst d) (snd d) S"
+    using holds by (simp only: parts(2) on_values[OF source reference parts(1)]; blast)
+  show "retained_clause_result E S p" unfolding retained_clause_result_def
+    by (rule exI[of _ F], rule exI[of _ u], rule exI[of _ r], rule exI[of _ Q], rule exI[of _ d], rule exI[of _ f])
+      (use parts actual in blast)
+next
+  assume "retained_clause_result E S p"
+  then obtain F u r Q d f where parts: "environment_value_presents F f"
+    "p=package_subject_argument f (use_data_term u) (Payload_Term r) (definition_site_value d)"
+    "native_package_at F u r Q" "d\<in>system_definitions Q"
+    "environment_included E F" "native_single_clause_at F (fst d) (snd d) S"
+    unfolding retained_clause_result_def by blast
+  show "(370,p)\<in>positive_meaning (retained_clause_system e v)"
+    by (simp only: parts(2) on_values[OF source reference parts(1)]) (use parts(3-6) in blast)
+qed
+
+theorem native_checker:
+  assumes source: "environment_value_presents E e" and reference: "schema_reference_presents S v"
+  shows "\<exists>C :: local_address option artifact_environment. \<exists>cu Q d.
+    closed_native_package_at C cu [] Q \<and> native_package_environment C cu []=C \<and>
+    d\<in>system_definitions Q \<and>
+    (\<forall>p. schema_call_formed Q d p \<longleftrightarrow> term_formed p) \<and>
+    (\<forall>p. (d,p)\<in>positive_meaning Q \<longleftrightarrow> retained_clause_result E S p)"
+proof -
+  obtain g :: "nat\<Rightarrow>local_address option definition_site"
+    and C :: "local_address option artifact_environment" and cu Q where compiled:
+    "inj_on g (system_definitions (retained_clause_system e v))"
+    "closed_native_package_at C cu [] Q" "native_package_environment C cu []=C"
+    "system_alpha_variant (rename_system g (retained_clause_system e v)) Q"
+    "positive_meaning Q=map_prod g id ` positive_meaning (retained_clause_system e v)"
+    using program_compilation_total[OF formed] by (elim exE conjE) (rule that; assumption)
+  have member: "370\<in>system_definitions (retained_clause_system e v)" by simp
+  have entry: "g 370\<in>system_definitions Q"
+    using compiled(4) member unfolding system_alpha_variant_def renamed_system_definitions by blast
+  have call: "schema_call_formed Q (g 370) p \<longleftrightarrow> term_formed p" for p
+    by (simp only: compiled_system_call_boundary[OF formed compiled(1,4) member] calls; simp)
+  have meaning: "(g 370,p)\<in>positive_meaning Q \<longleftrightarrow> retained_clause_result E S p" for p
+    by (simp only: compiled_system_meaning_at[OF compiled(1) member compiled(5)] exact[OF source reference])
+  show ?thesis by (rule exI[of _ C], rule exI[of _ cu], rule exI[of _ Q], rule exI[of _ "g 370"])
+    (use compiled(2,3) entry call meaning in blast)
+qed
+
+end
+
+
+section \<open>Every actual retained installation has an admitted complete presentation\<close>
+
+theorem retained_clause_presentations_total:
+  fixes F :: "local_address option artifact_environment"
+  assumes source: "environment_value_presents E e" and included: "environment_included E F"
+    and package: "native_package_at F u r Q" and member: "d\<in>system_definitions Q"
+    and read: "native_single_clause_at F (fst d) (snd d) S"
+  shows "\<exists>f v. environment_value_presents F f \<and> schema_reference_presents S v \<and>
+    (370,package_subject_argument f (use_data_term u) (Payload_Term r) (definition_site_value d))
+      \<in>positive_meaning (retained_clause_system e v)"
+proof -
+  have formed: "environment_formed F"
+    using native_package_projection(1)[OF package] by (simp add: native_package_formed_def)
+  obtain f where target: "environment_value_presents F f"
+    using environment_value_presents_total[OF formed] by blast
+  obtain a where schema: "native_schema_at F (fst d) a S"
+    using native_single_clause_schema[OF read] by blast
+  obtain v where reference: "schema_reference_presents S v"
+    using native_schema_reference_total[OF schema] by blast
+  interpret reader: retained_clause_reader e v
+    by (rule retained_clause_reader.intro)
+      (use environment_value_presents_formed[OF source] schema_reference_presents_formed[OF reference] in auto)
+  have admitted: "(370,package_subject_argument f (use_data_term u) (Payload_Term r) (definition_site_value d))
+      \<in>positive_meaning (retained_clause_system e v)"
+    by (simp only: reader.on_values[OF source reference target]) (use package member included read in blast)
+  show ?thesis using target reference admitted by blast
+qed
+
+text \<open>
+  The source environment and complete expected schema reference are fixed
+  before future operands. Three existing operations read the actual proposed
+  package entry, retain the entire original environment, and check the whole
+  definition. The installed program is recovered from its complete package;
+  its domain is not supplied as a substitute for its clauses or meanings.
+
+  This generic checker applies to any schema. Its source-retention condition
+  prevents the same callee coordinates from silently referring to changed
+  source artifacts. It does not decide whether an independently required
+  condition has been adequately expressed by that schema.
+\<close>
+
+end
