theories/Retained_Clause_Execution.thy
@@ -1,0 +1,112 @@
+theory Retained_Clause_Execution
+  imports Finite_Retained_Clause_Admission Factor_Finite_Equality_Source
+begin
+
+section \<open>Actual finite source changes keep their complete material\<close>
+
+definition finite_variable_artifact :: finite_exact_artifact where
+  "finite_variable_artifact=finite_equality_artifact\<lparr>finite_structure:=
+    (finite_structure finite_equality_artifact)\<lparr>finite_incidence:=
+      ffilter (\<lambda>(r,s,t). r\<noteq>[11]) (finite_incidence (finite_structure finite_equality_artifact))
+        |\<union>| {|([11],[11],[10])|}\<rparr>\<rparr>"
+
+definition finite_variable_schema :: "local_address option finite_native_schema" where
+  "finite_variable_schema=finite_equality_schema\<lparr>finite_schema_conclusion:=Finite_Variable [10]\<rparr>"
+
+definition finite_guard_artifact :: finite_exact_artifact where
+  "finite_guard_artifact=finite_variable_artifact\<lparr>
+    finite_structure:=(finite_structure finite_variable_artifact)\<lparr>
+      finite_carrier:=finite_carrier (finite_structure finite_variable_artifact) |\<union>|
+        fset_of_list (map (\<lambda>n. [n]) [26..<34]),
+      finite_incidence:=finite_incidence (finite_structure finite_variable_artifact) |\<union>|
+        fset_of_list (map (\<lambda>(r,s,t). ([r],[s],[t]))
+          [(14,26,27),(27,28,30),(27,29,31),(28,28,29),(30,30,32),(30,32,33),(31,31,10)])\<rparr>,
+    finite_data:=(finite_data finite_variable_artifact)\<lparr>finite_bindings:={|([33],[1])|}\<rparr>\<rparr>"
+
+definition finite_guard_schema :: "local_address option finite_native_schema" where
+  "finite_guard_schema=finite_variable_schema\<lparr>
+    finite_schema_premises:={|([26],(None,[1]),Finite_Variable [10])|}\<rparr>"
+
+definition finite_guard_source :: "bool \<Rightarrow> local_address option finite_artifact_environment" where
+  "finite_guard_source b=finite_enumerated_environment
+    [(None,if b then finite_variable_artifact else finite_equality_artifact)] []"
+
+definition finite_guard_environment :: "bool \<Rightarrow> local_address option finite_artifact_environment" where
+  "finite_guard_environment b=finite_enumerated_environment
+    [(None,if b then finite_variable_artifact else finite_equality_artifact),(Some [1],finite_guard_artifact)]
+    [((Some [1],[32]),None)]"
+
+definition finite_equality_extension :: "bool \<Rightarrow> local_address option finite_artifact_environment" where
+  "finite_equality_extension b=finite_enumerated_environment
+    [(None,finite_equality_artifact),(Some [9],finite_enumerated_artifact [[]] [] [] [])]
+    (if b then [((Some [9],[]),None)] else [])"
+
+definition finite_equality_changed_source :: "bool \<Rightarrow> local_address option finite_artifact_environment" where
+  "finite_equality_changed_source malformed=finite_enumerated_environment
+    [(None,finite_equality_artifact\<lparr>finite_structure:=(finite_structure finite_equality_artifact)\<lparr>
+      finite_carrier:=(if malformed then finite_carrier (finite_structure finite_equality_artifact) |-| {|[10]|}
+        else finsert [26] (finite_carrier (finite_structure finite_equality_artifact)))\<rparr>\<rparr>)] []"
+
+type_synonym retained_clause_control =
+  "local_address option finite_artifact_environment \<times> local_address option finite_native_schema \<times>
+    local_address option finite_artifact_environment \<times> local_address option \<times> local_address \<times>
+    local_address option definition_site"
+
+definition retained_clause_control :: "nat \<Rightarrow> retained_clause_control" where
+  "retained_clause_control n=(let C=finite_equality_environment; S=finite_equality_schema in
+    if n=0 then (C,S,C,None,[0],(None,[1])) else
+    if n=1 then (C,S,finite_equality_extension False,None,[0],(None,[1])) else
+    if n=2 then (C,S,finite_equality_changed_source False,None,[0],(None,[1])) else
+    if n=3 then (C,finite_variable_schema,C,None,[0],(None,[1])) else
+    if n=4 then (C,S,C,None,[0],(None,[8])) else
+    if n=5 then (C,S,C,None,[6],(None,[1])) else
+    if n=6 then (C,S,finite_enumerated_environment [] [],None,[0],(None,[1])) else
+    if n=7 then (C,S,finite_equality_changed_source True,None,[0],(None,[1])) else
+    if n=8 then (finite_equality_extension False,S,C,None,[0],(None,[1])) else
+    if n=9 then (finite_equality_extension True,S,finite_equality_extension True,None,[0],(None,[1])) else
+    if n=10 then (finite_equality_extension True,S,finite_equality_extension False,None,[0],(None,[1])) else
+    if n=11 then (C,finite_guard_schema,C,None,[0],(None,[1])) else
+    if n=12 then (C,finite_guard_schema,finite_guard_environment False,Some [1],[0],(Some [1],[1])) else
+    if n=13 then (C,finite_guard_schema,finite_guard_environment True,Some [1],[0],(Some [1],[1])) else
+      (finite_guard_source True,finite_guard_schema,finite_guard_environment True,Some [1],[0],(Some [1],[1])))"
+
+definition finite_retained_clause_observations where
+  "finite_retained_clause_observations C S D u r d=(let
+    source=finite_environment_formed C; target=finite_environment_formed D;
+    included=finite_environment_included C D;
+    programs=finite_native_package_readings D u r;
+    member=fBex programs (\<lambda>P. d |\<in>| finite_system_definitions P);
+    clause=finite_single_clause_at D (fst d) (snd d) S in
+    (sorted_list_of_fset (fimage (\<lambda>P. sorted_list_of_fset (finite_system_definitions P)) programs),
+      [source,target,included,member,clause,source \<and> included \<and> member \<and> clause]))"
+
+lemma finite_retained_clause_observation_equation:
+  "snd (finite_retained_clause_observations C S D u r d)=
+    [finite_environment_formed C,finite_environment_formed D,finite_environment_included C D,
+      finite_package_member D u r d,finite_single_clause_at D (fst d) (snd d) S,
+      finite_retained_clause_admitted C S D u r d]"
+  by (simp add: finite_retained_clause_observations_def finite_package_member_def finite_retained_clause_admitted_def Let_def)
+
+definition retained_clause_control_report where
+  "retained_clause_control_report n=(case retained_clause_control n of (C,S,D,u,r,d) \<Rightarrow>
+    ((finite_environment_artifact_rows C,sorted_list_of_fset (finite_environment_bindings C)),S,
+      (finite_environment_artifact_rows D,sorted_list_of_fset (finite_environment_bindings D)),u,r,d,
+      finite_retained_clause_observations C S D u r d))"
+
+export_code retained_clause_control_report finite_schema_conclusion finite_schema_premises finite_schema_materials
+  Finite_Variable Finite_Pattern_Payload Finite_Pattern_Pair Finite_Pattern_Target
+  fset set nat_of_integer integer_of_nat in SML module_name Retained_Clause_Execution file_prefix retained_clause_execution
+
+text \<open>
+  The input index selects the complete source, expected schema, candidate
+  environment, package root, and definition site through the displayed map.
+  Every reported condition is computed by its proved finite operation. The
+  report retains both complete environment tables and the recovered domain.
+
+  The last three controls use one unchanged guard calling the actual source
+  at None,[1]. Only that source clause changes between equality and acceptance
+  of every formed argument. The original source is required by control 13;
+  control 14 independently declares the changed source instead.
+\<close>
+
+end
